fix more FFIs

src/goose_lang/ffi/append_log_ffi.v
@@ -25,25 +25,25 @@ Section recoverable.
 
   Context {ext:ext_op}.
 
-  Definition openΣ : transition state (Σ*loc) :=
-    bind (reads id) (λ rs, match rs.(world) with
+  Definition openΣ : transition (state*global_state) (Σ*loc) :=
+    bind (reads id) (λ '(rs,g), match rs.(world) with
                            | Opened s l => ret (s,l)
                            | _ => undefined
                            end).
 
-  Definition modifyΣ (f:Σ -> Σ) : transition state unit :=
-    bind openΣ (λ '(s, l), modify (set world (λ _, Opened (f s) l))).
+  Definition modifyΣ (f:Σ -> Σ) : transition (state*global_state) unit :=
+    bind openΣ (λ '(s, l), modify (prod_map (set world (λ _, Opened (f s) l)) id)).
 
   (* TODO: generalize to a transition to construct the initial value, using a zoom *)
-  Definition initTo (init:Σ) (l:loc) : transition state unit :=
-    bind (reads id) (λ rs, match rs.(world) with
-                           | UnInit => modify (set world (fun _ => Opened init l))
+  Definition initTo (init:Σ) (l:loc) : transition (state*global_state) unit :=
+    bind (reads id) (λ '(rs,g), match rs.(world) with
+                           | UnInit => modify (prod_map (set world (fun _ => Opened init l)) id)
                            | _ => undefined
                            end).
 
-  Definition open (l:loc) : transition state Σ :=
-    bind (reads id) (λ rs, match rs.(world) with
-                           | Closed s => bind (modify (set world (fun _ => Opened s l)))
+  Definition open (l:loc) : transition (state*global_state) Σ :=
+    bind (reads id) (λ '(rs,g), match rs.(world) with
+                           | Closed s => bind (modify (prod_map (set world (fun _ => Opened s l)) id))
                                              (fun _ => ret s)
                            | _ => undefined
                            end).
@@ -119,7 +119,7 @@ Section log.
 
   Existing Instances r_mbind r_fmap.
 
-  Definition read_slice (t:ty) (v:val): transition state (list val) :=
+  Definition read_slice {state} (t:ty) (v:val): transition state (list val) :=
     match v with
     | PairV (#(LitLoc l)) (PairV #(LitInt sz) #(LitInt cap)) =>
       (* TODO: implement *)
@@ -138,19 +138,19 @@ Section log.
   (* TODO: implement *)
   Definition to_block (l: list val): option disk.Block := None.
 
-  Definition allocIdent: transition state loc :=
+  Definition allocIdent: transition (state*global_state) loc :=
     l ← allocateN 1;
-    modify (set heap <[l := Free #()]>);;
+    modify (prod_map (set heap <[l := Free #()]>) id);;
     ret l.
 
-  Definition log_step (op:LogOp) (v:val) : transition state val :=
+  Definition log_step (op:LogOp) (v:val) : transition (state*global_state) val :=
     match op, v with
     | GetOp, PairV (LitV (LitLoc logPtr)) (LitV (LitInt a)) =>
       openΣ ≫= λ '(log, logPtr_),
       check (logPtr = logPtr_);;
       b ← unwrap (log !! int.nat a);
       l ← allocateN 4096;
-      modify (state_insert_list l (disk.Block_to_vals b));;
+      modify (prod_map (state_insert_list l (disk.Block_to_vals b)) id);;
       ret $ #(LitLoc l)
     | ResetOp, LitV (LitLoc logPtr) =>
       openΣ ≫= λ '(_, logPtr_),
@@ -539,7 +539,7 @@ Instance logG0 : logG Σ := refinement_spec_ffiG.
     repeat match goal with
         | _ => progress simplify_map_eq/= (* simplify memory stuff *)
         | H : to_val _ = Some _ |- _ => apply of_to_val in H
-        | H : head_step ?e _ _ _ _ _ |- _ =>
+        | H : head_step ?e _ _ _ _ _ _ _ |- _ =>
           try (is_var e; fail 1); (* inversion yields many goals if [e] is a variable
      and can thus better be avoided. *)
           inversion H; subst; clear H
@@ -549,19 +549,19 @@ Instance logG0 : logG Σ := refinement_spec_ffiG.
           rewrite Heq in H1
         end.
 
-Lemma ghost_step_init_stuck E j K {HCTX: LanguageCtx K} σ:
+Lemma ghost_step_init_stuck E j K {HCTX: LanguageCtx K} σ g:
   nclose sN_inv ⊆ E →
   (σ.(@world _ log_spec_ffi_model.(@spec_ffi_model_field)) ≠ UnInit) →
   j ⤇ K (ExternalOp (ext := @spec_ext_op_field log_spec_ext) InitOp #()) -∗
   source_ctx (CS := spec_crash_lang) -∗
-  source_state σ -∗
+  source_state σ g -∗
   |NC={E}=> False.
 Proof.
   iIntros (??) "Hj Hctx H".
   iMod (ghost_step_stuck with "Hj Hctx H") as "[]".
   { eapply stuck_ExternalOp; first (by eauto).
     apply head_irreducible_not_atomically; [ by inversion 1 | ].
-    intros ?????.
+    intros ??????.
     repeat (inv_head_step; simpl in *; repeat monad_inv).
     destruct (σ.(world)); try congruence;
     repeat (inv_head_step; simpl in *; repeat monad_inv).
@@ -569,19 +569,19 @@ Proof.
   { solve_ndisj. }
 Qed.
 
-Lemma ghost_step_open_stuck E j K {HCTX: LanguageCtx K} σ:
+Lemma ghost_step_open_stuck E j K {HCTX: LanguageCtx K} σ g:
   nclose sN_inv ⊆ E →
   (∀ vs, σ.(@world _ log_spec_ffi_model.(@spec_ffi_model_field)) ≠ Closed vs) →
   j ⤇ K (ExternalOp (ext := @spec_ext_op_field log_spec_ext) OpenOp #()) -∗
   source_ctx (CS := spec_crash_lang) -∗
-  source_state σ -∗
+  source_state σ g -∗
   |NC={E}=> False.
 Proof.
   iIntros (??) "Hj Hctx H".
   iMod (ghost_step_stuck with "Hj Hctx H") as "[]".
   { eapply stuck_ExternalOp; first (by eauto).
     apply head_irreducible_not_atomically; [ by inversion 1 | ].
-    intros ?????.
+    intros ??????.
     repeat (inv_head_step; simpl in *; repeat monad_inv).
     destruct (σ.(world)); try congruence;
     repeat (inv_head_step; simpl in *; repeat monad_inv); eauto.
@@ -599,7 +599,7 @@ Lemma log_closed_init_false vs E j K {HCTX: LanguageCtx K}:
   False.
 Proof.
   iIntros (?) "(#Hctx&#Hstate) Hclosed_frag Hentries Hj".
-  iInv "Hstate" as (σ) "(>H&Hinterp)" "Hclo".
+  iInv "Hstate" as (σ g) "(>H&Hinterp)" "Hclo".
   iDestruct "Hinterp" as "(>Hσ&>Hffi&Hrest)".
   iDestruct (log_ctx_unify_closed with "[$] [$] [$]") as %Heq; subst.
   iMod (ghost_step_init_stuck with "[$] [$] [$]") as "[]".
@@ -615,7 +615,7 @@ Lemma log_opened_init_false l E j K {HCTX: LanguageCtx K}:
   False.
 Proof.
   iIntros (?) "(#Hctx&#Hstate) Hopened Hj".
-  iInv "Hstate" as (σ) "(>H&Hinterp)" "Hclo".
+  iInv "Hstate" as (σ g) "(>H&Hinterp)" "Hclo".
   iDestruct "Hinterp" as "(>Hσ&>Hffi&Hrest)".
   simpl.
   iDestruct (log_ctx_unify_opened with "[$] [$]") as %Heq; subst.
@@ -632,7 +632,7 @@ Lemma log_init_init_false E j K {HCTX: LanguageCtx K} j' K' {HCTX': LanguageCtx 
   False.
 Proof.
   iIntros (?) "(#Hctx&#Hstate) Hj Hj'".
-  iInv "Hstate" as (σ) "(>H&Hinterp)" "Hclo".
+  iInv "Hstate" as (σ g) "(>H&Hinterp)" "Hclo".
   iDestruct "Hinterp" as "(>Hσ&>Hffi&Hrest)".
   iEval (simpl) in "Hffi".
   destruct σ.(world) eqn:Heq; rewrite Heq; try (iDestruct "Hffi" as %[]).
@@ -665,14 +665,14 @@ Lemma log_init_open_false E j K {HCTX: LanguageCtx K} j' K' {HCTX': LanguageCtx 
   False.
 Proof.
   iIntros (?) "(#Hctx&#Hstate) Hj Hj'".
-  iInv "Hstate" as (σ) "(>H&Hinterp)" "Hclo".
+  iInv "Hstate" as (σ g) "(>H&Hinterp)" "Hclo".
   iDestruct "Hinterp" as "(>Hσ&>Hffi&Hrest)".
   iEval (simpl) in "Hffi".
   destruct σ.(world) eqn:Heq; rewrite Heq; try (iDestruct "Hffi" as %[]).
   - iMod (ghost_step_stuck with "Hj' Hctx H") as "[]".
     { eapply stuck_ExternalOp; first (by eauto).
       apply head_irreducible_not_atomically; [ by inversion 1 | ].
-      intros ?????. by repeat (inv_head_step; simpl in H3; repeat monad_inv).
+      intros ??????. by repeat (inv_head_step; simpl in H3; repeat monad_inv).
     }
     { solve_ndisj. }
   - iMod (ghost_step_init_stuck with "Hj [$] [$]") as "[]".
@@ -693,7 +693,7 @@ Lemma ghost_step_log_init E j K {HCTX: LanguageCtx K}:
   ∃ (l: loc), j ⤇ K (#l, #true)%V ∗ log_open l ∗ log_frag [].
 Proof.
   iIntros (?) "(#Hctx&#Hstate) Huninit_frag Hvals Hj".
-  iInv "Hstate" as (σ) "(>H&Hinterp)" "Hclo".
+  iInv "Hstate" as (σ g) "(>H&Hinterp)" "Hclo".
   iDestruct "Hinterp" as "(>Hσ&>Hffi&Hrest)".
   iDestruct (log_ctx_unify_uninit with "[$] [$]") as %Heq.
   iMod (ghost_step_lifting with "Hj Hctx H") as "(Hj&H&_)".
@@ -715,7 +715,7 @@ Proof.
   { apply (not_elem_of_dom (D := gset loc)). by apply fresh_locs_fresh. }
   { auto. }
   iMod ("Hclo" with "[Hσ Hvals_auth H Hrest]") as "_".
-  { iNext. iExists _. iFrame "H".  iFrame. iFrame "Hopen". rewrite fresh_alloc_equiv_null_non_alloc. iFrame. }
+  { iNext. iExists _, _. iFrame "H".  iFrame. iFrame "Hopen". rewrite fresh_alloc_equiv_null_non_alloc. iFrame. }
   iModIntro. iExists _. iFrame "Hopen". iFrame.
 Qed.
 
@@ -728,7 +728,7 @@ Lemma log_uninit_open_false vs E j K {HCTX: LanguageCtx K}:
   False.
 Proof.
   iIntros (?) "(#Hctx&#Hstate) Hclosed_frag Hentries Hj".
-  iInv "Hstate" as (σ) "(>H&Hinterp)" "Hclo".
+  iInv "Hstate" as (σ g) "(>H&Hinterp)" "Hclo".
   iDestruct "Hinterp" as "(>Hσ&>Hffi&Hrest)".
   iDestruct (log_ctx_unify_uninit with "[$] [$]") as %Heq; subst.
   iMod (ghost_step_open_stuck with "[$] [$] [$]") as "[]".
@@ -744,7 +744,7 @@ Lemma log_opened_open_false l E j K {HCTX: LanguageCtx K}:
   False.
 Proof.
   iIntros (?) "(#Hctx&#Hstate) Hopened Hj".
-  iInv "Hstate" as (σ) "(>H&Hinterp)" "Hclo".
+  iInv "Hstate" as (σ g) "(>H&Hinterp)" "Hclo".
   iDestruct "Hinterp" as "(>Hσ&>Hffi&Hrest)".
   simpl.
   iDestruct (log_ctx_unify_opened with "[$] [$]") as %Heq; subst.
@@ -761,7 +761,7 @@ Lemma log_open_open_false E j K {HCTX: LanguageCtx K} j' K' {HCTX': LanguageCtx 
   False.
 Proof.
   iIntros (?) "(#Hctx&#Hstate) Hj Hj'".
-  iInv "Hstate" as (σ) "(>H&Hinterp)" "Hclo".
+  iInv "Hstate" as (σ g) "(>H&Hinterp)" "Hclo".
   iDestruct "Hinterp" as "(>Hσ&>Hffi&Hrest)".
   iEval (simpl) in "Hffi".
   destruct σ.(world) eqn:Heq; rewrite Heq; try (iDestruct "Hffi" as %[]).
@@ -796,7 +796,7 @@ Lemma ghost_step_log_open E j K {HCTX: LanguageCtx K} vs:
   ∃ (l: loc), j ⤇ K #l%V ∗ log_open l ∗ log_frag vs.
 Proof.
   iIntros (?) "(#Hctx&#Hstate) Huninit_frag Hvals Hj".
-  iInv "Hstate" as (σ) "(>H&Hinterp)" "Hclo".
+  iInv "Hstate" as (σ g) "(>H&Hinterp)" "Hclo".
   iDestruct "Hinterp" as "(>Hσ&>Hffi&Hrest)".
   iDestruct (log_ctx_unify_closed with "[$] [$] [$]") as %Heq.
   iMod (ghost_step_lifting with "Hj Hctx H") as "(Hj&H&_)".
@@ -818,7 +818,7 @@ Proof.
   { apply (not_elem_of_dom (D := gset loc)). by apply fresh_locs_fresh. }
   { auto. }
   iMod ("Hclo" with "[Hσ Hvals_auth H Hrest]") as "_".
-  { iNext. iExists _. iFrame "H".  iFrame. iFrame "Hopen". rewrite fresh_alloc_equiv_null_non_alloc. iFrame. }
+  { iNext. iExists _, _. iFrame "H".  iFrame. iFrame "Hopen". rewrite fresh_alloc_equiv_null_non_alloc. iFrame. }
   iModIntro. iExists _. iFrame "Hopen". iFrame.
 Qed.
 
@@ -832,18 +832,18 @@ Lemma ghost_step_log_reset E j K {HCTX: LanguageCtx K} l vs:
   j ⤇ K #()%V ∗log_frag [].
 Proof.
   iIntros (?) "(#Hctx&#Hstate) #Hopen Hvals Hj".
-  iInv "Hstate" as (σ) "(>H&Hinterp)" "Hclo".
+  iInv "Hstate" as (σ g) "(>H&Hinterp)" "Hclo".
   iDestruct "Hinterp" as "(>Hσ&>Hffi&Hrest)".
   iDestruct (log_ctx_unify_opened with "[$] [$]") as %Heq.
   destruct Heq as (vs'&Heq).
   iMod (ghost_step_lifting with "Hj Hctx H") as "(Hj&H&_)".
-  { apply head_prim_step_trans. repeat (eauto || monad_simpl || rewrite Heq || econstructor). }
+  { apply head_prim_step_trans. repeat (eauto || monad_simpl || rewrite Heq || econstructor || simpl). }
   { solve_ndisj. }
   simpl. rewrite Heq.
   iDestruct "Hffi" as "(Huninit_auth&Hvals_auth)".
   iMod (log_state_update [] with "[$] [$]") as "(Hvals_auth&?)".
   iMod ("Hclo" with "[Hσ Hvals_auth H Hrest]") as "_".
-  { iNext. iExists _. iFrame "H". iFrame. iFrame "Hopen". }
+  { iNext. iExists _, _. iFrame "H". iFrame. iFrame "Hopen". }
   iModIntro. iFrame.
 Qed.
 
